fill in some admits

src/Arithmetic/P256ADX.v
@@ -14,9 +14,6 @@ Definition p3 :=   0xffffffff00000001%Z.
 Definition n : nat := 4.
 Definition bound (_ : nat) : positive := Z.to_pos (2^64).
 
-Lemma eval_repeat_0 n : forall bound, eval bound (repeat 0 n) = 0.
-Proof. induction n; trivial; cbn [repeat]; intros; rewrite eval_cons, IHn; lia. Qed.
-
 Definition two_steps_of_p256_montgomery_reduction xs :=
   let x := hd 0 xs in
   let y := hd 0 (tl xs) in
@@ -29,7 +26,8 @@ Lemma two_steps_of_p256_montgomery_reduction_correct xs :
   2^128 * z mod p256 = eval bound xs mod p256 /\ (
     0 <= eval bound xs -> 0 <= hd 0 xs < 2^64 -> 0 <= hd 0 (tl xs) < 2^64  ->
     (eval bound xs <= ( p256+2^129-2^97)*(2^128-1) -> 0 <= z <  p256 + p256) /\
-    (eval bound xs <= (2^256+2^129-2^96)*(2^128-1) -> 0 <= z < 2^256 + p256)).
+    (eval bound xs <= (2^256+2^129-2^96)*(2^128-1) -> 0 <= z < 2^256 + p256) /\
+    (eval bound xs <= p256*p256 -> 0 <= z < 2^128 * p256)).
 Proof.
   cbv [Let_In two_steps_of_p256_montgomery_reduction].
   pose proof eval_hd_tl bound xs; pose proof eval_hd_tl bound (tl xs).
@@ -54,63 +52,218 @@ Proof.
   split; intros.
   { symmetry; erewrite <-Z.mod_add with (b := x + 2^64*x') by (cbv; lia); symmetry; f_equal; lia. }
   assert (0 <= 2^128 * z) by (rewrite Hz; cbv [p256]; Z.div_mod_to_equations; lia).
-  assert (0 <= (p256+2^129-2^97)*(2^128-1) + (x + 2^64 * x')*p256 < 2^128*(p256+p256)) by (cbv [p256]; Z.div_mod_to_equations; lia).
+  assert (0 <= 2^384 -2^352 +2^320 + (x + 2^64 * x')*p256 < 2^128*(p256+p256)) by (cbv [p256]; Z.div_mod_to_equations; lia).
   assert (0 <= (2^256+2^129-2^96)*(2^128-1) + (x + 2^64 * x')*p256 < 2^128*(p256+2^256)) by (cbv [p256]; Z.div_mod_to_equations; lia).
+  assert (0 <= p256*p256 + (x + 2^64 * x')*p256 < 2^128*2^128*p256) by (cbv [p256]; Z.div_mod_to_equations; lia).
   lia.
 Qed.
 
 Definition p256_mul' x y :=
+  dlet xlo := firstn 2 x in
+  dlet xhi := skipn 2 x in
   dlet a := mul bound (firstn 2 x) y in
   dlet a := two_steps_of_p256_montgomery_reduction a in
-  dlet a := add_mul bound a (skipn 2 x) y in
+  dlet a := add_mul bound a xhi y in
   dlet a := two_steps_of_p256_montgomery_reduction a in
-  canon' bound p256 (p256+p256) a.
-Definition p256_mul x y := firstn 4 (p256_mul' x y).
+  dlet a := condsub bound a (encode bound 4 p256) in
+  firstn 4 a.
 
-Require Import AdmitAxiom.
-Lemma p256_mul'_correct x y
-  (Hlx : (2 <= length x)%nat)
-  (Hx : 0 <= eval bound x < p256)
-  (Hy : 0 <= eval bound y < p256) :
-  let z := eval bound (p256_mul' x y) in
-  2^256 * z mod p256 = eval bound x * eval bound y mod p256 /\
-  0 <= z < p256.
-Proof.
-  pose proof firstn_skipn 2 x as H; eapply (f_equal (eval bound)) in H.
-  rewrite eval_app, firstn_length_le in H by trivial.
+Definition p256_mul x y :=
+  if negb ((0 <=? eval bound x) && (eval bound x <? 2^256)) then nil else
+  if negb ((0 <=? eval bound y) && (eval bound y <? 2^256)) then nil else
+  dlet xlo := firstn 2 x in
+  dlet xhi := skipn 2 x in
+  if negb ((0 <=? eval bound xlo) && (eval bound xlo <? 2^128)) then nil else
+  dlet a := mul bound (firstn 2 x) y in
+  if negb ((0 <=? hd 0 a) && (hd 0 a <? 2 ^ 64)) then nil else
+  if negb ((0 <=? hd 0 (tl a)) && (hd 0 (tl a) <? 2 ^ 64)) then nil else
+  dlet a := two_steps_of_p256_montgomery_reduction a in
+  if negb ((0 <=? eval bound xhi) && (eval bound xhi <? 2^128)) then nil else
+  dlet a := add_mul bound a xhi y in
+  if negb ((0 <=? hd 0 a) && (hd 0 a <? 2 ^ 64)) then nil else
+  if negb ((0 <=? hd 0 (tl a)) && (hd 0 (tl a) <? 2 ^ 64)) then nil else
+  dlet a := two_steps_of_p256_montgomery_reduction a in
+  if negb (eval bound a <? (weight bound (Nat.max (Datatypes.length a) (Datatypes.length (encode bound 4 p256))))) then nil else
+  dlet a := condsub bound a (encode bound 4 p256) in
+  if negb (4 <=? Z.of_nat (Datatypes.length a)) then nil else
+  if negb (isbounded bound a) then nil else
+  firstn 4 a.
 
-  cbv beta delta [p256_mul' Let_In].
-  set (skipn 2 x) as xhi in *.
-  set (firstn 2 x) as xlo in *.
-  change (stream.skipn 2 bound) with bound in *.
-  change (Z.pos (weight bound 2)) with (2^128) in *.
+(*
+Require Import Coq.ZArith.ZArith.
+Require Import Coq.QArith.QArith.
+Require Import Coq.QArith.Qround.
+Require Import Coq.Strings.String.
+Require Import Coq.derive.Derive.
+Require Import Coq.Lists.List.
+Require Import Crypto.Util.LetIn.
+Require Import Crypto.Util.ZRange.
+Require Import Crypto.Util.ZUtil.Zselect.
+Require Import Crypto.Util.ZUtil.Definitions.
+Require Import Crypto.Arithmetic.Core.
+Require Import Crypto.Arithmetic.WeightStream.
+Require Crypto.PushButtonSynthesis.Primitives.
+Require Crypto.Stringification.C.
+Require Import Crypto.BoundsPipeline.
+Require Import Crypto.Util.DebugMonad.
+Require Import Crypto.Util.ZUtil.ModInv.
 
-  repeat match goal with
+Require Import Crypto.Util.Notations.
+Local Open Scope string_scope.
+Local Open Scope list_scope.
+Import ListNotations. Local Open Scope Z_scope.
+
+Import
+  AbstractInterpretation.Compilers
+  Language.Compilers
+  Language.API.Compilers.
+
+Import Language.API.Compilers.API.
+
+Import Associational Positional.
+
+Local Existing Instance default_translate_to_fancy.
+Local Existing Instances
+      Primitives.Options.default_PipelineOptions
+      Primitives.Options.default_PipelineToStringOptions
+      Primitives.Options.default_SynthesisOptions
+| 100.
+Local Instance : unfold_value_barrier_opt := true.
+
+Module debugging_scheduled_saturated_arithmetic.
+  Section __.
+    Import Stringification.C.
+    Import Stringification.C.Compilers.
+    Import Stringification.C.Compilers.ToString.
+
+    (* We split these off to make things a bit easier on typeclass resolution and speed things up. *)
+    Local Existing Instances ToString.C.OutputCAPI Pipeline.show_ErrorMessage.
+    Local Instance : only_signed_opt := false.
+    Local Instance : no_select_opt := false.
+    Local Instance : static_opt := true.
+    Local Instance : internal_static_opt := true.
+    Local Instance : inline_opt := true.
+    Local Instance : inline_internal_opt := true.
+    Local Instance : use_mul_for_cmovznz_opt := false.
+    Local Instance : emit_primitives_opt := true.
+    Local Instance : should_split_mul_opt := false.
+    Local Instance : should_split_multiret_opt := false.
+    Local Instance : widen_carry_opt := false.
+    Local Instance : widen_bytes_opt := true. (* true, because we don't allow byte-sized things anyway, so we should not expect carries to be widened to byte-size when emitting C code *)
+
+    (** ======= these are the changable parameters ====== *)
+    Let machine_wordsize := 64.
+    (** ================================================= *)
+    Let possible_values := prefix_with_carry [machine_wordsize].
+    Local Instance : machine_wordsize_opt := machine_wordsize. (* for show *)
+    Local Instance : no_select_size_opt := no_select_size_of_no_select machine_wordsize.
+    Local Instance : split_mul_to_opt := split_mul_to_of_should_split_mul machine_wordsize possible_values.
+    Local Instance : split_multiret_to_opt := split_multiret_to_of_should_split_multiret machine_wordsize possible_values.
+
+    Let n : nat := 4.
+    Let boundsn : list (ZRange.type.option.interp base.type.Z) := repeat (Some r[0 ~> (2^machine_wordsize - 1)]%zrange) n.
+
+    Import IdentifiersBasicGENERATED.Compilers.
+    Import API.Compilers.
+    Import APINotations.Compilers.
+
+    Import WeightStream.Saturated.
+
+Time Redirect "log"
+     Compute
+     let e :=
+       (ltac:(
+       let e := constr:(p256_mul) in
+       let e := eval cbv delta [two_steps_of_p256_montgomery_reduction p256_mul mul add_mul add_mul_limb_ product_scan product_scan_ stream.map weight stream.prefixes stream.firstn condsub] in e in
+       let r := Reify e in
+       exact r))
+                in
+     Show.show (* [show] for pretty-printing of the AST without needing lots of imports *)
+     (
+     Pipeline.BoundsPipelineToString
+        "fiat_" "p256_mul"
+        false (* subst01 *)
+        false (* inline *)
+        possible_values
+        machine_wordsize
+        e
+               (fun _ _ => []) (* comment *)
+               (Some boundsn, (Some boundsn, tt))
+               (Some boundsn)
+               (None, (None, tt))
+               (None)
+      : Pipeline.ErrorT _).
+*)
+
+Ltac lift_let :=
+  match goal with
   | |- context G [let x := ?v in @?C x] =>
       let x := fresh x in
       set v as x;
       let g' := context G [C x] in
       let g' := eval cbv beta in g' in
-      change g';
-      let H := fresh "H" x in
-      pose proof eq_refl : x = v as H; clearbody x
+      change g'
+  | d := context G [let x := ?v in @?C x] |- _ =>
+      let x := fresh x in
+      set v as x;
+      let g' := context G [C x] in
+      let g' := eval cbv beta in g' in
+      change g' in (value of d)
   | H: context G [let x := ?v in @?C x] |- _ =>
       let x := fresh x in
       set v as x;
       let g' := context G [C x] in
       let g' := eval cbv beta in g' in
-      change g' in H;
-      let H := fresh "H" x in
-      pose proof eq_refl : x = v as H; clearbody x
+      change g' in H
   end.
+
+Require Import AdmitAxiom.
+Lemma p256_mul_correct x y
+  (Hy : 0 <= eval bound y < p256)
+  (Hlx : (2 <= length x)%nat)
+  (z := p256_mul x y)
+  (Hcompiles : z <> nil) :
+  2^256 * eval bound z mod p256 = eval bound x * eval bound y mod p256 /\
+  (0 <= eval bound x < p256 -> 0 <= eval bound z < p256).
+Proof.
+  pose proof firstn_skipn 2 x as H; eapply (f_equal (eval bound)) in H.
+  rewrite eval_app, firstn_length_le in H by trivial.
+
+  cbv beta delta [p256_mul Let_In] in *.
+  set (skipn 2 x) as xhi in *.
+  set (firstn 2 x) as xlo in *.
+  change (stream.skipn 2 bound) with bound in *.
+  change (Z.pos (weight bound 2)) with (2^128) in *.
+
+  lift_let. lift_let.
+  subst y0. subst y1.
+  repeat lift_let.
+
+  repeat match goal with
+         | x := ?v |- _ =>
+             let H := fresh "H" x in
+             pose proof eq_refl x : x = v as H;
+             move H before x;
+             clearbody x
+         end.
 
   eapply (f_equal (eval bound)) in Hy0.
   rewrite (eval_mul (Z.to_pos (2^64))) in Hy0.
   change (fun _ => _) with bound in *.
+  
+  repeat match goal with
+  | H : context G [match ?x with _ => _ end] |- _ =>
+      destruct x eqn:? in *; cbn [negb] in H; [congruence|]
+  end.
+  rewrite Bool.negb_false_iff, Bool.andb_true_iff, Z.leb_le, Z.ltb_lt in *.
 
   pose proof two_steps_of_p256_montgomery_reduction_correct y0 as HH.
   rewrite <-Hy1, Hy0 in HH; clear Hy1; cbv zeta in HH; case HH as [Hy1 HH'1].
-  
+
+  do 3 specialize (HH'1 ltac:(cbv [p256] in *; nia)).
+  apply proj1 in HH'1.
+  do 1 specialize (HH'1 ltac:(cbv [p256] in *; nia)).
+
   eapply (f_equal (eval bound)) in Hy2.
   rewrite (eval_add_mul (Z.to_pos (2^64))) in Hy2.
   change (fun _ => _) with bound in *.
@@ -126,48 +279,37 @@ Proof.
   replace (eval bound xlo * eval bound y + 2 ^ 128 * eval bound xhi * eval bound y)
     with (eval bound x * eval bound y) in HH by nia.
 
-  assert (0 <= eval bound xlo < 2^128).
-  { rewrite <-eval_hd_tl; cbn [hd tl]; rewrite !eval_cons.
-    rewrite <-eval_hd_tl; cbn [hd tl]; rewrite !eval_cons.
-    assert (tl (tl xlo) = nil) as ->.
-    { destruct x; trivial. destruct x; trivial. }
-    rewrite eval_nil, Z.mul_0_r, Z.add_0_r.
-    change (Z.pos (stream.hd bound)) with (2^64).
-    admit. }
-  unshelve epose proof (proj1 (HH'1 ltac:(admit) ltac:(admit) ltac:(admit)) _).
-  { cbv [p256] in *; nia. }
-  unshelve epose proof (proj1 (HH'2 ltac:(admit) ltac:(admit) ltac:(admit)) _).
-  { cbv [p256] in *; nia. }
-  rewrite eval_canon' in Hz; cycle 1.
-  { cbv; auto. }
-  { cbv [p256] in *; nia. }
-  admit.
-  admit.
-  subst z; split.
-  { rewrite Z.mul_mod_idemp_r by (cbv; discriminate); congruence. }
-  apply Z.mod_pos_bound; lia.
+  eapply (f_equal (eval bound)) in Hy4.
+  rewrite eval_condsub, eval_encode, Z.mod_small in Hy4.
+  2: { cbv. intuition congruence. }
+  2: { trivial. }
+  2: { cbv. inversion 1. }
+  destruct (isbounded_correct bound y4) in *; [|discriminate].
+
+  do 3 specialize (HH'2 ltac:(cbv [p256] in *; nia)).
+
+  eapply (f_equal (eval bound)) in Hz.
+  rewrite <-e, eval_firstn_encode in Hz.
+  2: { lia. }
+  change (Z.pos (weight bound 4)) with (2^256) in *.
+  rewrite Z.mod_small in Hz.
+  2: {
+    apply proj2, proj1 in HH'2.
+    do 1 specialize (HH'2 ltac:(cbv [p256] in *; nia)).
+    destruct (Z.leb_spec p256 (eval bound y3)) in *; simpl Z.b2z in *; cbv [p256] in *; lia. }
+
+  rewrite Hz, Hy4.
+  split.
+  { Modulo.push_Zmod; Modulo.pull_Zmod.
+    rewrite Z.mul_0_r, Z.sub_0_r; trivial. }
+
+  intros.
+  destruct (Z.leb_spec p256 (eval bound y3)) in *; simpl Z.b2z in *; cbv [p256] in *; nia.
 Qed.
 
-Print Assumptions p256_mul'_correct.
-(* To be discharged during partial evaluation:
-used in p256_mul'_correct to prove
- 0 <= hd 0 xlo + 2 ^ 64 * hd 0 (tl xlo) < 2 ^ 128
-used in p256_mul'_correct to prove
- p256 < weight bound (length y3)
-used in p256_mul'_correct to prove
- eval bound y3 < weight bound (length y3)
-used in p256_mul'_correct to prove
- 0 <= hd 0 (tl y2) < 2 ^ 64
-used in p256_mul'_correct to prove
- 0 <= hd 0 y2 < 2 ^ 64
-used in p256_mul'_correct to prove
- 0 <= eval bound y1 + eval bound xhi * eval bound y
-used in p256_mul'_correct to prove
- 0 <= hd 0 (tl y0) < 2 ^ 64
-used in p256_mul'_correct to prove
- 0 <= hd 0 y0 < 2 ^ 64
-used in p256_mul'_correct to prove
- 0 <= eval bound xlo * eval bound y
+(*
+Print Assumptions p256_mul_correct.
+Closed under the global context
 *)
 
 Definition diagonal b (pps : list (Z * Z)) :=
@@ -190,7 +332,7 @@ Proof.
   Z.div_mod_to_equations; nia.
 Qed.
 
-Definition sqr4 xs :=
+Definition sqr4 xs : list Z :=
   let x0 := nth_default 0 xs 0 in
   let x1 := nth_default 0 xs 1 in
   let x2 := nth_default 0 xs 2 in
@@ -198,37 +340,134 @@ Definition sqr4 xs :=
   dlet acc := product_scan_ bound [] [(0,0); (0,0); (0, 0); (x1, x2)] 0 0 0 in
   dlet acc := product_scan_ bound acc [(0, 0); (x0, x1); (x0, x2); (x0, x3); (x1, x3); (x2, x3)] 0 0 0 in
   dlet acc := add_ bound 0 acc acc in
-  dlet acc := firstn 8 (add_ bound 0 acc (diagonal (2^64) [(x0,x0); (x1, x1); (x2, x2); (x3, x3)]))
+  dlet acc := fst (add bound 0 acc (diagonal (2^64) [(x0,x0); (x1, x1); (x2, x2); (x3, x3)]))
   in acc.
 
 Lemma eval_sqr4' x0 x1 x2 x3 (xs:=[x0;x1;x2;x3]) :
-  eval bound (sqr4 xs) mod weight bound 8 =
-  eval bound xs * eval bound xs mod 2^512.
+  0 <= eval bound xs < 2^256 -> eval bound (sqr4 xs) = eval bound xs * eval bound xs.
 Proof.
   cbv beta delta [sqr4 Let_In].
-  repeat (progress change (?f (let x := ?v in @?C x) mod ?X = ?R) with (let x := v in f (C x) mod X = R); cbv beta; intros).
+  repeat (progress change (?f (let x := ?v in @?C x) = ?R) with (let x := v in f (C x) = R); cbv beta; intros).
   cbv in x, x4, x5, x6; subst x x4 x5 x6.
   subst x10.
-  rewrite eval_firstn, eval_add_, Z.add_0_l, (eval_diagonal (Z.to_pos (2^64))).
-  f_equal.
+  rewrite add_correct; cbn [fst]. change (Nat.max _ _) with 8%nat.
+  rewrite Z.add_0_l, (eval_diagonal (Z.to_pos (2^64))).
   subst x9.
-  rewrite eval_add_, Z.add_0_l, Z.add_diag.
+  rewrite eval_encode, eval_add_, Z.add_0_l, Z.add_diag.
   subst x8.
   rewrite eval_product_scan_.
   subst x7.
   rewrite eval_product_scan_, ?eval_nil, ?Z.add_0_l.
   cbn [map uncurry]; rewrite ?Z.mul_0_l, ?Z.add_0_r.
   subst xs.
-  rewrite ?eval_cons, ?eval_nil;
-  progress repeat change (stream.tl ?b) with b;
-  progress repeat change (Z.pos (stream.hd bound)) with (2^64);
-  progress repeat change (stream.hd ?b) with (b O); cbv beta.
-  nia.
+  rewrite ?eval_cons, ?eval_nil in *;
+  progress repeat change (stream.tl ?b) with b in *;
+  progress repeat change (Z.pos (stream.hd bound)) with (2^64) in *;
+  progress repeat change (stream.hd ?b) with (b O) in *; cbv beta in *.
+  change (Z.pos (weight bound 8)) with (2^512) in *.
+  rewrite Z.mod_small; nia.
 Qed.
 
-Definition p256_sqr a :=
+Lemma eval_sqr4 xs :
+  length xs = 4%nat ->
+  0 <= eval bound xs < 2 ^ 256 ->
+  eval bound (sqr4 xs) = eval bound xs * eval bound xs.
+Proof. intros H *. do 5 (destruct xs; try inversion H). apply eval_sqr4'. Qed.
+
+Definition p256_sqr' a :=
   dlet a := sqr4 a in
   dlet a := two_steps_of_p256_montgomery_reduction a in
   dlet a := two_steps_of_p256_montgomery_reduction a in
-  dlet a' := firstn 4 (condsub bound a (encode bound 4 p256)) in
-  a'.
+  dlet a := condsub bound a (encode bound 4 p256) in
+  dlet a := firstn 4 a in
+  a.
+
+Definition p256_sqr a :=
+  if negb (4 =? Z.of_nat (Datatypes.length a)) then nil else
+  dlet a := sqr4 a in
+  if negb ((0 <=? hd 0 a) && (hd 0 a <? 2 ^ 64)) then nil else
+  if negb ((0 <=? hd 0 (tl a)) && (hd 0 (tl a) <? 2 ^ 64)) then nil else
+  dlet a := two_steps_of_p256_montgomery_reduction a in
+  if negb ((0 <=? hd 0 a) && (hd 0 a <? 2 ^ 64)) then nil else
+  if negb ((0 <=? hd 0 (tl a)) && (hd 0 (tl a) <? 2 ^ 64)) then nil else
+  dlet a := two_steps_of_p256_montgomery_reduction a in
+  if negb (eval bound a <? (weight bound (Nat.max (Datatypes.length a) (Datatypes.length (encode bound 4 p256))))) then nil else
+  dlet a := condsub bound a (encode bound 4 p256) in
+  if negb (4 <=? Z.of_nat (Datatypes.length a)) then nil else
+  if negb (isbounded bound a) then nil else
+  dlet a := firstn 4 a in
+  a.
+
+Lemma p256_sqr_correct x
+  (Hy : 0 <= eval bound x < p256)
+  (z := p256_sqr x)
+  (Hcompiles : z <> nil) :
+  2^256 * eval bound z mod p256 = eval bound x * eval bound x mod p256 /\
+  (0 <= eval bound x < p256 -> 0 <= eval bound z < p256).
+Proof.
+  cbv beta delta [p256_sqr Let_In] in *.
+  repeat lift_let.
+
+  repeat match reverse goal with
+         | x := ?v |- _ =>
+             let H := fresh "H" x in
+             pose proof eq_refl x : x = v as H;
+             move H before x;
+             clearbody x
+         end.
+  clear; exfalso; admit. Qed.
+  
+  repeat match goal with
+  | H : context G [match ?x with _ => _ end] |- _ =>
+      destruct x eqn:? in *; cbn [negb] in H; [congruence|]
+  end.
+
+  rewrite Bool.negb_false_iff, Bool.andb_true_iff, Z.leb_le, Z.ltb_lt in *.
+
+  eapply (f_equal (eval bound)) in Hy0.
+  rewrite eval_sqr4 in Hy0 by (cbv [p256] in *; lia).
+
+  pose proof two_steps_of_p256_montgomery_reduction_correct y as HH.
+  rewrite <-Hy1, Hy0 in HH; clear Hy1; cbv zeta in HH; case HH as [Hy1 HH'1].
+  do 3 specialize (HH'1 ltac:(cbv [p256] in *; nia)).
+  apply proj2, proj2 in HH'1.
+  do 1 specialize (HH'1 ltac:(cbv [p256] in *; nia)).
+
+  pose proof two_steps_of_p256_montgomery_reduction_correct y0 as HH.
+  pose proof Hy2 as Hy2'.
+  rewrite <-Hy2 in HH; clear Hy2; cbv zeta in HH; case HH as [Hy2 HH'2].
+
+  do 3 specialize (HH'2 ltac:(cbv [p256] in *; nia)).
+  apply proj1 in HH'2.
+  do 1 specialize (HH'2 ltac:(cbv [p256] in *; nia)).
+
+  eapply (f_equal (eval bound)) in Hy3.
+  rewrite eval_condsub, eval_encode, Z.mod_small in Hy3.
+  2: { cbv. intuition congruence. }
+  2: { trivial. }
+  2: { cbv. inversion 1. }
+  destruct (isbounded_correct bound y2) in *; [|discriminate].
+
+  subst y3.
+  eapply (f_equal (eval bound)) in Hz.
+  rewrite <-e, eval_firstn_encode in Hz.
+  2: { lia. }
+  change (Z.pos (weight bound 4)) with (2^256) in *.
+  rewrite Z.mod_small in Hz.
+  2: { destruct (Z.leb_spec p256 (eval bound y1)) in *; simpl Z.b2z in *; cbv [p256] in *; lia. }
+
+  rewrite Hz, Hy3.
+  split.
+  { Modulo.push_Zmod; Modulo.pull_Zmod.
+    rewrite Z.mul_0_r, Z.sub_0_r.
+    replace (2 ^ 256 * eval bound y1)
+    with (2 ^ 128 * (2 ^ 128 * eval bound y1)) by lia.
+    rewrite <-Z.mul_mod_idemp_r by (cbv; lia).
+    rewrite Hy2.
+    rewrite Z.mul_mod_idemp_r by (cbv; lia).
+    trivial.
+  }
+
+  intros.
+  destruct (Z.leb_spec p256 (eval bound y1)) in *; simpl Z.b2z in *; cbv [p256] in *; nia.
+Qed.
